make dummy_cbor, cbor_map_entry manual constructors/destructors explicit

src/cbor/CBOR.SteelST.Type.fst
@@ -9,22 +9,6 @@ let cbor_map_entry = cbor_map_entry
 
 let cbor = cbor
 
-let dummy_cbor : cbor = CBOR_Case_Simple_value 0uy dummy_cbor_footprint
-
-let cbor_map_entry_key x = match x with
-| Mkcbor_map_entry k _ -> k
-
-let cbor_map_entry_value x = match x with
-| Mkcbor_map_entry _ v -> v
-
-let cbor_map_entry_key_value_inj
-  m1 m2
-= ()
-
-let mk_cbor_map_entry
-  k v
-= Mkcbor_map_entry k v
-
 let cbor_array_iterator_t = cbor_array_iterator_t
 
 let cbor_map_iterator_t = cbor_map_iterator_t
