src/cbor/impl/CBOR.SteelST.Match.fst
@@ -12,6 +12,22 @@ module LPS = LowParse.SteelST.SeqMatch
 module LW = LowParse.SteelST.L2ROutput.IntroElim
 module GR = Steel.ST.GhostReference
 
+let dummy_cbor : cbor = CBOR_Case_Simple_value 0uy dummy_cbor_footprint
+
+let cbor_map_entry_key x = match x with
+| Mkcbor_map_entry k _ -> k
+
+let cbor_map_entry_value x = match x with
+| Mkcbor_map_entry _ v -> v
+
+let cbor_map_entry_key_value_inj
+  m1 m2
+= ()
+
+let mk_cbor_map_entry
+  k v
+= Mkcbor_map_entry k v
+
 let prod_perm
   (p1 p2: perm)
 : Tot perm
